coq/stepverse/LabeledSet.v
@@ -1,0 +1,260 @@
+
+Require Export ssreflect.
+Require Export Coq.Classes.RelationClasses.
+Require Export Coq.Classes.Morphisms.
+
+Require Coq.Sorting.Sorted.
+Require Coq.Lists.List.
+
+Require structures.Option.
+Require Import structures.Sets.
+Require Import structures.Monad.
+Require structures.Vector.
+
+Require Import stepverse.label.
+Import LabelNotation.
+Require Export stepverse.result.
+
+Require Import Classical.
+
+Set Implicit Arguments.
+
+(* --------------------------------------------------------- *)
+(* --------------------------------------------------------- *)
+(*      Monadic type                                         *)
+(* --------------------------------------------------------- *)
+(* --------------------------------------------------------- *)
+
+(** The semantics of computations is a set of labeled results.  These sets
+   should be partial functions, i.e. there should be at most one result for
+   any label in the set. *)
+
+Definition M (A : Type) := (label * Result A) -> Prop.  
+
+Section PartialFunctions.
+
+Variable A : Type.
+
+Variable R : A -> A -> Prop.
+
+Context `{Equivalence A R} `{PartialOrder A R}.
+
+Import SetNotations.
+
+(** ** entries and entry approximations *)
+
+(* A pair of a label and result is an entry. *)
+
+Definition entry (A:Type) := (label * Result A)%type.
+
+Definition default_label {A} (r : Result A) := 
+  if R.isBottom r then Bot else Top.
+
+(* An entry is "finished" if the label does not contain Bot and the result is
+   not Bottom. *)
+
+(* this is the same as not containing Bot *)
+Definition label_finished (l : label) := 
+  forall l', l ⊑ l' -> l = l'.
+
+(* this used to be forall r', R.approx R r r' -> r = r'. 
+   However, with the introduction of approximation for values, 
+   this is no longer appropriate. *)
+(* this is the same as r <> Bottom *)
+Definition result_finished (r : Result A) := 
+  r <> Bottom.
+
+Definition entry_finished '((l,r) : entry A) := 
+  label_finished l /\ result_finished r.
+
+Definition entry_valid '((l,r) : entry A) := 
+  label_finished l <-> result_finished r.
+
+(* Entry approximation is pointwise *)
+
+Definition entry_approx '(l1,r1) '(l2, r2) : Prop := 
+  Label.approx l1 l2 /\ R.approx R r1 (r2 : Result A).
+
+(** ** set approximatation *)
+
+(* Because we will use these sets as the semantics of computations, we 
+   need to say what it means for one set to *approximate* another.
+
+   We have s1 ⊑ s2 when:
+
+      1. for every e in s1 that has finished (i.e. is Value or Wrong), 
+          a. e must be in s2 
+
+      2. if e has bottomed 
+          a. it could stay bottom, with a potentially bigger label
+          b. it could succeed, with a bigger label
+          c. it could fail and won't be in s2
+
+      3. if e is not in s1, i.e. fails
+          - then it should continue to fail, i.e. all bigger labels shouldn't be in s2
+
+   We can express 1 as is
+   Case 2 is trivial
+   we can express 3 using the contrapositive:
+            everything in s2 should be approximated by something in s1
+         
+We need (1) to know that successful values do not change with more fuel.
+We need (3) for the case of ONE: there won't be new "smaller" elements 
+when we add more fuel.
+*)
+
+Definition approx (s1 s2 : M A) : Prop := 
+  (* (1) We don't lose successful results. 
+     Everything that has finished in s1 is still present in s2. *)
+  (forall e, e ∈ s1 -> entry_finished e -> (e ∈ s2)) /\
+  (* (3) We don't make up results. 
+     Every entry in s2 is approximated by something from s1. *)
+  (forall e2, e2 ∈ s2 -> exists e1, (e1 ∈ s1) /\ entry_approx e1 e2).
+
+
+(** ** partial functions *)
+
+(* We can look up values in the set by label. This label can be exactly the 
+   same as the label in some entry, or it can be an extension of the label 
+   of an unfinished entry. *)
+
+Definition mapsto '(l,r) (s : M A) := 
+  exists l', ((l',r) ∈ s) /\ Label.approx l' l.
+
+
+(** ** !!!!! Classical logic !!!!! *)
+
+Lemma decide_mapsto : forall (s : M A) l,
+  (mapsto (l, Bottom) s) \/ not (mapsto (l, Bottom) s).
+intros. eapply classic. Qed.
+
+(* A set of pairs is a partial function if there is at most one mapping for
+   any key in the set. *)
+Definition partial_function (s : M A) := 
+  forall l r1 r2, mapsto (l,r1) s -> mapsto (l, r2) s -> r1 = r2.
+
+(* This predicate defines when a key is in the domain of 
+   the partial function *)
+Definition in_dom (s : M A) (l : label) : Prop := 
+  exists l' r, ((l', r) ∈ s) /\ Label.approx l' l.
+
+(** ** entry ordering, by labels only *)
+Definition entry_lt : (label * Result A) -> (label * Result A) -> Prop := 
+  fun '(l1,_) '(l2, _)=> Label.lt l1 l2.
+
+(* The canonical list of entries in a finite set *)
+Definition elements (s : M A) (l : list (label * Result A)) : Prop := 
+  (mem l = s) /\                        (* memberships are equal *)
+  @Sorted.LocallySorted _ entry_lt l.  (* the list is sorted by the labels *)
+
+(** ** Properties of partial_functions, approx, and labeled sets *)
+
+Lemma smaller_notpresent 
+  (a : label * Result A) (w : list (label * Result A)) :
+  List.Forall (entry_lt a) w ->  ~(List.In a w).
+Proof. destruct a. 
+       induction w.
+       intros h1 h2. inversion h2.
+       intros h1 h2. simpl in h2. 
+       inversion h1. subst.
+       destruct h2.
+       + subst. eapply Label.lt_irreflexive; eauto.
+       + apply IHw; eauto.
+Qed.
+
+Lemma exact_mapsto e (s : M A) : (e ∈ s) -> mapsto e s.
+Proof. 
+  move: e => [l r].
+  move=> in1.
+  exists l. split. auto. eapply Label.approx_refl.
+Qed.
+
+Lemma elements_functional {e: M A}{w1 w2 : list (label * Result A)} : 
+  elements e w1 -> elements e w2 -> w1 = w2.
+Proof.
+  unfold elements.
+  intros [M1 S1] [M2 S2].
+  rewrite <- Sorted.Sorted_LocallySorted_iff in S1.
+  rewrite <- Sorted.Sorted_LocallySorted_iff in S2.
+  have h: (mem w1 = mem w2). subst. auto.
+  clear M1 M2 e.
+  move: w2 h S1 S2.
+  induction w1.
+  - intros w2 h S1 S2.
+    destruct w2. auto. 
+    unfold mem in h.
+    admit.
+  - intros w2 h S1 S2.
+    destruct w2. admit.
+    apply Sorted.Sorted_extends in S1.
+    apply Sorted.Sorted_extends in S2.
+Admitted.
+
+Lemma partial_function_singleton {k}{r:Result A} : 
+   partial_function ⌈ (k , r) ⌉.
+ Proof. 
+   intros l r1 r2 [l1 [m1 a1]] [l2 [m2 a2]].
+   inversion m1. inversion m2. subst. auto.
+ Qed.
+
+Lemma entry_approx_label {l1 r1 l2 r2}: 
+  entry_approx (l1, r1) (l2, r2) -> Label.approx l1 l2.
+destruct r1; simpl; tauto.
+Qed.
+
+Lemma entry_approx_refl (e : label * Result A) : entry_approx e e.
+Proof. destruct e as [l r].
+       destruct r; simpl; split; eauto using Label.approx_refl, 
+       Equivalence_Reflexive. 
+Qed.
+
+Lemma entry_approx_trans (e1 e2 e3 : label * Result A) : 
+  entry_approx e1 e2 -> entry_approx e2 e3 -> entry_approx e1 e3.
+Proof. destruct e1 as [l1 r1]. destruct e2 as [l2 r2]. destruct e3 as [l3 r3]. 
+       destruct r1; destruct r2; simpl.
+Admitted.
+(*
+       eauto using Label.approx_trans. 
+       intros h1 [h2 e]. eauto using Label.approx_trans. 
+       intros h1 [h2 e]. eauto using Label.approx_trans. 
+       intros [h1 e] h2. discriminate.
+       intros [h1 e1] [h2 e2]. eauto using Label.approx_trans. 
+       intros [h1 e1] [h2 e2]. discriminate.
+       intros [h1 e1] h2. discriminate.
+       intros [h1 e1] h2. discriminate.
+       intros [h1 e1] [h2 e2]. inversion e1. subst. eauto using Label.approx_trans. 
+Qed. *)
+
+Lemma approx_refl (s : M A) : approx s s.
+  split. intros e eIn eFin. auto.
+  intros e2 e2In. exists e2. split. auto.
+  eapply entry_approx_refl.
+Qed.
+
+Lemma nonBottomIsFinished (r : Result A) : r <> Bottom -> result_finished r.
+  intros NE. unfold result_finished. auto.
+(*  intros r' RA.
+  destruct r; try done; simpl in RA; destruct r'; try done. f_equal. auto. *)
+Qed.
+
+Lemma bottomIsNotFinished : not (result_finished (@Bottom A)).
+  intros h. cbv in h. auto. 
+  (* have: (@Bottom A) = (@Wrong A). eapply h. simpl. done. done. *)
+Qed.
+
+Lemma approx_not_finished l l1 : 
+~ label_finished l ->
+  l1 ⊑ l ->
+  ~ label_finished l1.
+Admitted.
+
+Lemma label_finished_Br_inv1 l0 l1: label_finished (l0 ⋈ l1) -> label_finished l0.
+Admitted.
+Lemma label_finished_Br_inv2 l0 l1: label_finished (l0 ⋈ l1) -> label_finished l1.
+Admitted.
+Lemma Value_finished {a : A} : result_finished (Value a).
+Admitted.
+
+End PartialFunctions.
+
+#[export] Hint Unfold entry : core.
