coq/stepverse/result.v
@@ -1,0 +1,56 @@
+
+(* --------------------------------------------------------- *)
+(* --------------------------------------------------------- *)
+(*                     Result                                *)
+(* --------------------------------------------------------- *)
+(* --------------------------------------------------------- *)
+
+Inductive Result (A : Type) : Type := 
+  | Bottom : Result A       (* divergence *)
+  | Wrong  : Result A       (* runtime type error *)
+  | Value  : A -> Result A.
+
+Arguments Bottom {_}.
+Arguments Wrong {_}.
+Arguments Value  {_}.
+
+(* Note: *failure* is the absence of any result in the set so is not included
+   as a constructor in the result type.
+
+   This design simplifies the operation of "One" --- we only need to find the
+   result with the smallest label in the set, not the smallest label with a
+   nonfailing result.
+
+   The cost for not modelling failure is that it is difficult to say when one
+   *set* of results approximates another. Labeled bottoms can disappear when
+   given more fuel, because they could fail.  *)
+
+
+Module R. 
+
+Definition isWrong {A} (r : Result A) : bool := 
+  match r with | Wrong => true | _ => false end.
+Definition isBottom {A} (r: Result A) : bool := 
+  match r with | Bottom => true | _ => false end.
+Definition isValue {A} (r: Result A) : bool := 
+  match r with | Value _ => true | _ => false end.
+
+(* Parameterized by an approximation function for 
+   the value type *)
+Definition approx {A} (R : A -> A -> Prop) (r1 r2 : Result A) : Prop := 
+  match r1 , r2 with 
+  | Bottom , _ => True
+  | Wrong , Wrong => True
+  | Value w1 , Value w2 => R w1 w2
+  | _ , _ => False
+end.
+
+Definition approxb {A} (R : A -> A -> bool) (r1 : Result A) (r2 : Result A) : bool := 
+  match r1 , r2 with
+  | Value w1 , Value w2 => R w1 w2
+  | Wrong , Wrong => true
+  | Bottom , _ => true
+  | _ , _  => false
+  end.
+
+End R.
